\documentclass[12pt]{article}
\usepackage[pdftex]{graphicx}
\usepackage{amsmath}
\usepackage{amssymb}
\pagestyle{empty}
\author{Chris Camano: ccamano@sfsu.edu}
\title{MATH 310  Homework 1.1 }
\date{8/22/2022}

\topmargin -0.6in
\headsep 0.40in
\oddsidemargin 0.0in
\textheight 9.0in
\textwidth 6.5in

\newcommand{\econst}{\mathrm{e}}
\newcommand{\diff}{\mathrm{d}}
\newcommand{\dwrt}[1]{\frac{\diff}{\diff #1}}
%%%%%%Macros for 425%%%%%%%%%%%%%%%%%%%
\newcommand{\q}{\quad}
\newcommand{\tab}{\\\\}
\renewcommand{\labelenumi}{\alph{enumi})}
\newcommand{\sect}[1]{\section*{#1}}

%%%%%%Vector Spaces%%%%%%%%%%%%%%%%%%%
\newcommand{\R}{\mathbb{R}}
\newcommand{\C}{\mathbb{C}}
\newcommand{\F}{\mathbb{F}}
\newcommand{\rtwo}{\mathbb{R}^2}
\newcommand{\mxn}{{mxn}}

%%%%%%Sets and common phrases%%%%%%%%%
\newcommand{\Axb}{\textbf{Ax=b} }
\newcommand{\Axz}{\textbf{Ax=0} }
\newcommand{\dim}{\text{dim}}
\newcommand{\lc}{linear combination }
\newcommand{\let}{\text{Let }}
\newcommand{\tf}{\therefore}
%%%%%%%%%%%%%%%%%%%%%%%%%%%%%%%%%%%%%%%
\everymath={\displaystyle}


\begin{document}
\maketitle
\sect{1}
\begin{proof}
Prove that
\[
  \sum_{i=1}^ni^2=\frac{n(n+1)(2n+1)}{6}
\]
\begin{align*}
  &P(k)=\sum_{i=1}^ki^2=\frac{k(k+1)(2k+1)}{6}\\
  &P(k+1):\\
  &\sum_{i=1}^{k+1}i^2=\frac{k+1(k+1+1)(2(k+1)+1)}{6}\\\\
  &\frac{k(k+1)(2k+1)}{6}+(k+1)^2=\frac{k+1(k+2)(2k+3)}{6}\\\\
  &\frac{2k^3+9k^2+13k+6}{6}=\frac{2k^3+9k^2+13k+6}{6}
\end{align*}
\end{proof}
\sect{2}
Prove that :
\[
  \sum_{i=0}^ni^3=(\sum_{i=1}^ni)^2
\]
\begin{align*}
  &\sum_{i=0}^ni^3=(\frac{n(n+1)}{2})^2\\\\
  &\sum_{i=0}^ni^3=(\frac{n^2+n}{2})^2\\\\
  &\sum_{i=0}^ni^3=\frac{(n^2+n)^2}{4}\\\\
  &P(k)=\sum_{i=0}^ki^3=\frac{(k^2+k)^2}{4}\\\\
  &P(k+1):\\\\
  &\sum_{i=0}^{k+1}i^3=(\frac{((k+1)^2+k+1)^2}{4})\\\\
  &\frac{(k^2+k)^2}{4}+(k+1)^3=\frac{\left(k^2+3k+2\right)^2}{4}\\\\
  &\frac{k^4+6k^3+13k^2+12k+4}{4}=\frac{k^4+6k^3+13k^2+12k+4}{4}
\end{align*}
\sect{3}
\begin{proof}
  Prove that:
  \[
    x^n-y^n=(x-y) \sum_{i=1}^n x^{n-i}y^{i-1}
  \]
  Another representation of the sum that is easier to work with would be:
  \[
    x^n-y^n=(x-y) \sum_{i=0}^{k-1}x^iy^{k-1-i}
  \]
  \begin{align*}
    &P(k)=    x^k-y^k=(x-y) \sum_{i=0}^{k-1}x^iy^{k-1-i}\\\\
    &P(k)=    \frac{x^k-y^k}{(x-y) }=\sum_{i=0}^{k-1}x^iy^{k-1-i}\\\\
    &P(k+1):\\\\
    &P(k+1)=\frac{x^{k+1}-y^{k+1}}{(x-y) }=\sum_{i=0}^{k}x^iy^{k-i}\\\\
    &\frac{x^{k+1}-y^{k+1}}{(x-y) }=x^k+\sum_{i=0}^{k-1}x^iy^{k-i}\\\\
    &\frac{x^{k+1}-y^{k+1}}{(x-y) }=x^k+y\sum_{i=0}^{k-1}x^iy^{k-1-i}\\\\
    &\frac{x^{k+1}-y^{k+1}}{(x-y) }=x^k+y\left \frac{x^k-y^k}{(x-y) }\right\\\\
    & \frac{x^{k+1}-y^{k+1}}{(x-y) }=\frac{x^{k+1}-y^{k+1}}{(x-y) }
  \end{align*}
\end{proof}
\end{document}
